src/core-props/bir_extra_expsScript.sml
@@ -1,0 +1,405 @@
+open HolKernel Parse boolLib bossLib;
+open HolBACoreSimps
+open bir_expTheory bir_imm_expTheory bir_valuesTheory
+open bir_typing_expTheory bir_envTheory wordsTheory
+
+(* Some extra expressions that are sometimes useful. *)
+
+val _ = new_theory "bir_extra_exps";
+
+
+(*********)
+(* Align *)
+(*********)
+
+
+
+val BExp_Align_def = Define `BExp_Align sz p e =
+  (BExp_BinExp BIExp_And e (BExp_Const (n2bs (2 ** (size_of_bir_immtype sz) - (2 ** p)) sz)))`;
+
+
+val BExp_Align_vars_of = store_thm ("BExp_Align_vars_of",
+``!sz p e. bir_vars_of_exp (BExp_Align sz p e) = bir_vars_of_exp e``,
+SIMP_TAC (std_ss++holBACore_ss) [BExp_Align_def, pred_setTheory.UNION_EMPTY]);
+
+
+val BExp_Align_type_of = store_thm ("BExp_Align_type_of",
+``!sz p e. type_of_bir_exp (BExp_Align sz p e) =
+           if (type_of_bir_exp e = SOME (BType_Imm sz)) then
+               SOME (BType_Imm sz) else NONE``,
+
+REPEAT GEN_TAC >>
+SIMP_TAC (std_ss++holBACore_ss) [BExp_Align_def, type_of_bir_exp_def,
+  pairTheory.pair_case_thm] >>
+REPEAT CASE_TAC >> (
+  FULL_SIMP_TAC (std_ss++holBACore_ss) [bir_type_checker_DEFS]
+));
+
+
+val BExp_Align_eval = store_thm ("BExp_Align_eval",
+``!sz p e env. bir_eval_exp (BExp_Align sz p e) env =
+     case (sz, bir_eval_exp e env) of
+         (Bit1,  BVal_Imm (Imm1 w))  => BVal_Imm (Imm1 (align p w))
+       | (Bit8,  BVal_Imm (Imm8 w))  => BVal_Imm (Imm8 (align p w))
+       | (Bit16, BVal_Imm (Imm16 w)) => BVal_Imm (Imm16 (align p w))
+       | (Bit32, BVal_Imm (Imm32 w)) => BVal_Imm (Imm32 (align p w))
+       | (Bit64, BVal_Imm (Imm64 w)) => BVal_Imm (Imm64 (align p w))
+       | (_, _) => BVal_Unknown``,
+
+REPEAT GEN_TAC >>
+SIMP_TAC (std_ss++holBACore_ss) [BExp_Align_def, alignmentTheory.align_bitwise_and,
+  pairTheory.pair_case_thm, LSL_UINT_MAX] >>
+REPEAT CASE_TAC >> (
+   FULL_SIMP_TAC (std_ss++holBACore_ss++wordsLib.SIZES_ss) []
+));
+
+
+val align_AND_INTROS = save_thm ("align_AND_INTROS", let
+  val thm0 = prove (``!w:'a word p.
+     (MEM p (COUNT_LIST (dimindex (:'a)))) ==> (0 < p) ==>
+     (((w && n2w (dimword (:'a) - 2 ** p) = align p w)) /\
+      (((n2w (dimword (:'a) - 2 ** p) && w) = align p w)))``,
+   SIMP_TAC std_ss [alignmentTheory.align_bitwise_and, LSL_UINT_MAX] >>
+   METIS_TAC[wordsTheory.WORD_AND_COMM]);
+
+  val words_sizes = List.map (fn sz => fcpLib.index_type (Arbnum.fromInt sz))
+          bir_immSyntax.known_imm_sizes;
+  val thm2 = LIST_CONJ (List.map (fn sz => INST_TYPE [``:'a`` |-> sz] thm0) words_sizes)
+
+  val thm3 = SIMP_RULE (std_ss++wordsLib.SIZES_ss) [rich_listTheory.COUNT_LIST_compute,
+    rich_listTheory.COUNT_LIST_AUX_def_compute, DISJ_IMP_THM, listTheory.MEM,
+    FORALL_AND_THM, GSYM CONJ_ASSOC] thm2
+in thm3 end);
+
+
+(***********)
+(* Aligned *)
+(***********)
+
+val BExp_Aligned_def = Define `BExp_Aligned sz p e =
+   (BExp_BinPred BIExp_Equal
+      (BExp_BinExp BIExp_And e (BExp_Const (n2bs (2 ** p - 1) sz)))
+      (BExp_Const (n2bs 0 sz)))`
+
+val BExp_Aligned_vars_of = store_thm ("BExp_Aligned_vars_of",
+``!sz p e. bir_vars_of_exp (BExp_Aligned sz p e) = bir_vars_of_exp e``,
+SIMP_TAC (std_ss++holBACore_ss) [BExp_Aligned_def, pred_setTheory.UNION_EMPTY]);
+
+
+val BExp_Aligned_type_of = store_thm ("BExp_Aligned_type_of",
+``!sz p e. type_of_bir_exp (BExp_Aligned sz p e) =
+           if (type_of_bir_exp e = SOME (BType_Imm sz)) then
+               SOME BType_Bool else NONE``,
+
+REPEAT GEN_TAC >>
+SIMP_TAC (std_ss++holBACore_ss) [BExp_Aligned_def, type_of_bir_exp_def,
+  pairTheory.pair_case_thm] >>
+REPEAT CASE_TAC >> (
+  FULL_SIMP_TAC (std_ss++holBACore_ss) [bir_type_checker_DEFS]
+));
+
+val BExp_Aligned_eval = store_thm ("BExp_Aligned_eval",
+``!sz p e env. bir_eval_exp (BExp_Aligned sz p e) env =
+     case (sz, bir_eval_exp e env) of
+         (Bit1,  BVal_Imm (Imm1 w))  => BVal_Imm (bool2b (aligned p w))
+       | (Bit8,  BVal_Imm (Imm8 w))  => BVal_Imm (bool2b (aligned p w))
+       | (Bit16, BVal_Imm (Imm16 w)) => BVal_Imm (bool2b (aligned p w))
+       | (Bit32, BVal_Imm (Imm32 w)) => BVal_Imm (bool2b (aligned p w))
+       | (Bit64, BVal_Imm (Imm64 w)) => BVal_Imm (bool2b (aligned p w))
+       | (_, _) => BVal_Unknown``,
+
+REPEAT GEN_TAC >>
+SIMP_TAC (std_ss++holBACore_ss) [BExp_Aligned_def, alignmentTheory.aligned_bitwise_and] >>
+REPEAT CASE_TAC >> (
+   FULL_SIMP_TAC (std_ss++holBACore_ss) [
+     bir_bool_expTheory.bir_bin_exp_BOOL_OPER_EVAL]
+));
+
+
+
+
+(******************)
+(* Reverse Endian *)
+(******************)
+
+val reverse_endian16_def = Define `
+  reverse_endian16 (w:word16) =
+    (((((7 >< 0) w):word8) @@ (((16 >< 8) w):word8)) : word16)`
+
+val reverse_endian32_def = Define `
+ reverse_endian32 (w:word32) =
+     (((((7 :num) >< (0 :num)) w :word8) @@
+       (((((15 :num) >< (8 :num)) w :word8) @@
+        (((((23 :num) >< (16 :num)) w :word8) @@
+         (((31 :num) >< (24 :num)) w :word8))
+           :word16))
+          :word24))
+        :word32)`
+
+val reverse_endian64_def = Define `
+ reverse_endian64 (w:word64) =
+     (((((7 :num) >< (0 :num)) w :word8) @@
+       (((((15 :num) >< (8 :num)) w :word8) @@
+        (((((23 :num) >< (16 :num)) w :word8) @@
+         (((((31 :num) >< (24 :num)) w :word8) @@
+          (((((39 :num) >< (32 :num)) w :word8) @@
+           (((((47 :num) >< (40 :num)) w :word8) @@
+            (((((55 :num) >< (48 :num)) w :word8) @@
+             (((63 :num) >< (56 :num)) w :word8))
+           :word16))
+          :word24))
+        :word32))
+           :40 word))
+          :48 word))
+        :56 word)):word64)`;
+
+
+val reverse_endian16_id = store_thm ("reverse_endian16_id",
+``!w:word16. reverse_endian16 (reverse_endian16 w) = w``,
+
+Cases >>
+ONCE_REWRITE_TAC [fcpTheory.CART_EQ] >>
+FULL_SIMP_TAC (arith_ss++boolSimps.EQUIV_EXTRACT_ss++wordsLib.SIZES_ss) [fcpTheory.FCP_BETA,
+  reverse_endian16_def, word_bits_def, word_extract_def, w2w, word_concat_def, word_join_index]);
+
+
+val reverse_endian32_id = store_thm ("reverse_endian32_id",
+``!w:word32. reverse_endian32 (reverse_endian32 w) = w``,
+
+Cases >>
+ONCE_REWRITE_TAC [fcpTheory.CART_EQ] >>
+FULL_SIMP_TAC (arith_ss++boolSimps.EQUIV_EXTRACT_ss++wordsLib.SIZES_ss) [fcpTheory.FCP_BETA,
+  reverse_endian32_def, word_bits_def, word_extract_def, w2w, word_concat_def, word_join_index]);
+
+
+val reverse_endian64_id = store_thm ("reverse_endian64_id",
+``!w:word64. reverse_endian64 (reverse_endian64 w) = w``,
+
+Cases >>
+ONCE_REWRITE_TAC [fcpTheory.CART_EQ] >>
+FULL_SIMP_TAC (arith_ss++boolSimps.EQUIV_EXTRACT_ss++wordsLib.SIZES_ss) [fcpTheory.FCP_BETA,
+  reverse_endian64_def, word_bits_def, word_extract_def, w2w, word_concat_def, word_join_index]);
+
+
+
+
+val word_extract_byte_def = Define `word_extract_byte (w:'a word) (n:num) =
+  (w && ((n2w 255) << n))`
+
+
+
+val word_extract_byte_index = store_thm ("word_extract_byte_index",
+``!w:'a word m n. m < dimindex (:'a) ==>
+  ((word_extract_byte w n) ' m =
+  ((w ' m) /\ (n <= m) /\ (m < n + 8)))``,
+
+REPEAT STRIP_TAC >>
+ONCE_REWRITE_TAC [fcpTheory.CART_EQ] >>
+FULL_SIMP_TAC (arith_ss++boolSimps.EQUIV_EXTRACT_ss++wordsLib.SIZES_ss) [fcpTheory.FCP_BETA,
+  word_lsl_def, word_and_def, word_index, word_extract_byte_def] >>
+
+MP_TAC (Q.SPECL [`m-n`, `8`] bitTheory.BIT_EXP_SUB1) >>
+ASM_SIMP_TAC arith_ss []);
+
+
+
+
+val reverse_endian16_ALT_DEF = store_thm ("reverse_endian16_ALT_DEF",
+``!w:word16. reverse_endian16 w = (w >>> 8) || (w << 8)``,
+
+Cases >>
+ONCE_REWRITE_TAC [fcpTheory.CART_EQ] >>
+FULL_SIMP_TAC (arith_ss++boolSimps.EQUIV_EXTRACT_ss++wordsLib.SIZES_ss) [fcpTheory.FCP_BETA,
+  reverse_endian16_def, word_bits_def, word_extract_def, w2w, word_concat_def, word_join_index,
+  word_or_def, word_lsr_def, word_lsl_def] >>
+SIMP_TAC (arith_ss++boolSimps.LIFT_COND_ss) []);
+
+
+val reverse_endian32_ALT_DEF_aux = prove (
+``!w:word32. reverse_endian32 w = (w >>> 24) || (word_extract_byte (w >>> 8) 8) ||
+                                  (word_extract_byte (w << 8) 16) || (w << 24)``,
+
+GEN_TAC >>
+ONCE_REWRITE_TAC [fcpTheory.CART_EQ] >>
+FULL_SIMP_TAC (arith_ss++boolSimps.EQUIV_EXTRACT_ss++wordsLib.SIZES_ss) [fcpTheory.FCP_BETA,
+  reverse_endian32_def, word_bits_def, word_extract_def, w2w, word_concat_def, word_join_index,
+  word_or_def, word_and_def, word_extract_byte_index, word_lsl_def, word_lsr_def] >>
+SIMP_TAC (arith_ss++boolSimps.LIFT_COND_ss) []);
+
+val reverse_endian32_ALT_DEF = save_thm ("reverse_endian32_ALT_DEF",
+  SIMP_RULE (std_ss++wordsLib.SIZES_ss) [word_extract_byte_def, word_lsl_n2w] reverse_endian32_ALT_DEF_aux);
+
+
+val reverse_endian64_ALT_DEF_aux = prove (
+``!w:word64. reverse_endian64 w = (w >>> 56) || (word_extract_byte (w >>> 40) 8) ||
+                                  (word_extract_byte (w >>> 24) 16) ||
+                                  (word_extract_byte (w >>> 8) 24) ||
+                                  (word_extract_byte (w << 8) 32) ||
+                                  (word_extract_byte (w << 24) 40) ||
+                                  (word_extract_byte (w << 40) 48) ||
+                                  (w << 56)``,
+
+GEN_TAC >>
+ONCE_REWRITE_TAC [fcpTheory.CART_EQ] >>
+FULL_SIMP_TAC (arith_ss++boolSimps.EQUIV_EXTRACT_ss++wordsLib.SIZES_ss) [fcpTheory.FCP_BETA,
+  reverse_endian64_def, word_bits_def, word_extract_def, w2w, word_concat_def, word_join_index,
+  word_or_def, word_and_def, word_extract_byte_index, word_lsl_def, word_lsr_def] >>
+SIMP_TAC (arith_ss++boolSimps.LIFT_COND_ss) []);
+
+
+val reverse_endian64_ALT_DEF = save_thm ("reverse_endian64_ALT_DEF",
+  SIMP_RULE (std_ss++wordsLib.SIZES_ss) [word_extract_byte_def, word_lsl_n2w] reverse_endian64_ALT_DEF_aux);
+
+
+val BExp_reverse_endian64_def = Define `BExp_reverse_endian64 e1 =
+      (BExp_BinExp BIExp_Or
+        (BExp_BinExp BIExp_RightShift e1 (BExp_Const (Imm64 56w)))
+        (BExp_BinExp BIExp_Or
+           (BExp_BinExp BIExp_And
+              (BExp_BinExp BIExp_RightShift e1 (BExp_Const (Imm64 40w)))
+              (BExp_Const (Imm64 65280w)))
+           (BExp_BinExp BIExp_Or
+              (BExp_BinExp BIExp_And
+                 (BExp_BinExp BIExp_RightShift e1
+                    (BExp_Const (Imm64 24w)))
+                 (BExp_Const (Imm64 0xFF0000w)))
+              (BExp_BinExp BIExp_Or
+                 (BExp_BinExp BIExp_And
+                    (BExp_BinExp BIExp_RightShift e1
+                       (BExp_Const (Imm64 8w)))
+                    (BExp_Const (Imm64 0xFF000000w)))
+                 (BExp_BinExp BIExp_Or
+                    (BExp_BinExp BIExp_And
+                       (BExp_BinExp BIExp_LeftShift e1
+                          (BExp_Const (Imm64 8w)))
+                       (BExp_Const (Imm64 0xFF00000000w)))
+                    (BExp_BinExp BIExp_Or
+                       (BExp_BinExp BIExp_And
+                          (BExp_BinExp BIExp_LeftShift e1
+                             (BExp_Const (Imm64 24w)))
+                          (BExp_Const (Imm64 0xFF0000000000w)))
+                       (BExp_BinExp BIExp_Or
+                          (BExp_BinExp BIExp_And
+                             (BExp_BinExp BIExp_LeftShift e1
+                                (BExp_Const (Imm64 40w)))
+                             (BExp_Const (Imm64 0xFF000000000000w)))
+                          (BExp_BinExp BIExp_LeftShift e1
+                             (BExp_Const (Imm64 56w))))))))))`
+
+val BExp_reverse_endian32_def = Define `BExp_reverse_endian32 e1 =
+     (BExp_BinExp BIExp_Or
+        (BExp_BinExp BIExp_RightShift e1 (BExp_Const (Imm32 24w)))
+        (BExp_BinExp BIExp_Or
+           (BExp_BinExp BIExp_And
+              (BExp_BinExp BIExp_RightShift e1 (BExp_Const (Imm32 8w)))
+              (BExp_Const (Imm32 65280w)))
+           (BExp_BinExp BIExp_Or
+              (BExp_BinExp BIExp_And
+                 (BExp_BinExp BIExp_LeftShift e1
+                    (BExp_Const (Imm32 8w)))
+                 (BExp_Const (Imm32 0xFF0000w)))
+              (BExp_BinExp BIExp_LeftShift e1
+                 (BExp_Const (Imm32 24w))))))`
+
+val BExp_reverse_endian16_def = Define `BExp_reverse_endian16 e1 =
+     (BExp_BinExp BIExp_Or
+        (BExp_BinExp BIExp_RightShift e1 (BExp_Const (Imm16 8w)))
+        (BExp_BinExp BIExp_LeftShift e1 (BExp_Const (Imm16 8w))))`
+
+
+
+val BExp_reverse_endian16_vars_of = store_thm ("BExp_reverse_endian16_vars_of",
+``!e. bir_vars_of_exp (BExp_reverse_endian16 e) = bir_vars_of_exp e``,
+SIMP_TAC (std_ss++holBACore_ss) [BExp_reverse_endian16_def, pred_setTheory.UNION_EMPTY,
+  pred_setTheory.UNION_IDEMPOT]);
+
+
+
+val BExp_reverse_endian32_vars_of = store_thm ("BExp_reverse_endian32_vars_of",
+``!e. bir_vars_of_exp (BExp_reverse_endian32 e) = bir_vars_of_exp e``,
+SIMP_TAC (std_ss++holBACore_ss) [BExp_reverse_endian32_def, pred_setTheory.UNION_EMPTY,
+  pred_setTheory.UNION_IDEMPOT]);
+
+
+val BExp_reverse_endian64_vars_of = store_thm ("BExp_reverse_endian64_vars_of",
+``!e. bir_vars_of_exp (BExp_reverse_endian64 e) = bir_vars_of_exp e``,
+SIMP_TAC (std_ss++holBACore_ss) [BExp_reverse_endian64_def, pred_setTheory.UNION_EMPTY,
+  pred_setTheory.UNION_IDEMPOT]);
+
+
+val BExp_reverse_endian16_type_of = store_thm ("BExp_reverse_endian16_type_of",
+``!e. type_of_bir_exp (BExp_reverse_endian16 e) =
+      (if (type_of_bir_exp e = SOME (BType_Imm Bit16)) then SOME (BType_Imm Bit16) else NONE)``,
+
+REPEAT GEN_TAC >>
+SIMP_TAC (std_ss++holBACore_ss) [BExp_reverse_endian16_def, type_of_bir_exp_def,
+  pairTheory.pair_case_thm] >>
+REPEAT CASE_TAC >> (
+  FULL_SIMP_TAC (std_ss++holBACore_ss) [bir_type_checker_DEFS]
+));
+
+val BExp_reverse_endian32_type_of = store_thm ("BExp_reverse_endian32_type_of",
+``!e. type_of_bir_exp (BExp_reverse_endian32 e) =
+      (if (type_of_bir_exp e = SOME (BType_Imm Bit32)) then SOME (BType_Imm Bit32) else NONE)``,
+
+REPEAT GEN_TAC >>
+SIMP_TAC (std_ss++holBACore_ss) [BExp_reverse_endian32_def, type_of_bir_exp_def,
+  pairTheory.pair_case_thm] >>
+REPEAT CASE_TAC >> (
+  FULL_SIMP_TAC (std_ss++holBACore_ss) [bir_type_checker_DEFS]
+));
+
+val BExp_reverse_endian64_type_of = store_thm ("BExp_reverse_endian64_type_of",
+``!e. type_of_bir_exp (BExp_reverse_endian64 e) =
+      (if (type_of_bir_exp e = SOME (BType_Imm Bit64)) then SOME (BType_Imm Bit64) else NONE)``,
+
+REPEAT GEN_TAC >>
+SIMP_TAC (std_ss++holBACore_ss) [BExp_reverse_endian64_def, type_of_bir_exp_def,
+  pairTheory.pair_case_thm] >>
+REPEAT CASE_TAC >> (
+  FULL_SIMP_TAC (std_ss++holBACore_ss) [bir_type_checker_DEFS]
+));
+
+
+val BExp_reverse_endian16_eval = store_thm ("BExp_reverse_endian16_eval",
+``!e env. bir_eval_exp (BExp_reverse_endian16 e) env =
+     case (bir_eval_exp e env) of
+       | (BVal_Imm (Imm16 w)) => BVal_Imm (Imm16 (reverse_endian16 w))
+       | _ => BVal_Unknown``,
+
+REPEAT GEN_TAC >>
+SIMP_TAC (std_ss++holBACore_ss) [BExp_reverse_endian16_def] >>
+REPEAT CASE_TAC >> (
+  FULL_SIMP_TAC (std_ss++holBACore_ss++wordsLib.SIZES_ss) [reverse_endian16_ALT_DEF,
+    wordsTheory.word_shift_bv]
+));
+
+val BExp_reverse_endian32_eval = store_thm ("BExp_reverse_endian32_eval",
+``!e env. bir_eval_exp (BExp_reverse_endian32 e) env =
+     case (bir_eval_exp e env) of
+       | (BVal_Imm (Imm32 w)) => BVal_Imm (Imm32 (reverse_endian32 w))
+       | _ => BVal_Unknown``,
+
+REPEAT GEN_TAC >>
+SIMP_TAC (std_ss++holBACore_ss) [BExp_reverse_endian32_def] >>
+REPEAT CASE_TAC >> (
+  FULL_SIMP_TAC (std_ss++holBACore_ss++wordsLib.SIZES_ss) [reverse_endian32_ALT_DEF,
+    wordsTheory.word_shift_bv]
+));
+
+
+val BExp_reverse_endian64_eval = store_thm ("BExp_reverse_endian64_eval",
+``!e env. bir_eval_exp (BExp_reverse_endian64 e) env =
+     case (bir_eval_exp e env) of
+       | (BVal_Imm (Imm64 w)) => BVal_Imm (Imm64 (reverse_endian64 w))
+       | _ => BVal_Unknown``,
+
+REPEAT GEN_TAC >>
+SIMP_TAC (std_ss++holBACore_ss) [BExp_reverse_endian64_def] >>
+REPEAT CASE_TAC >> (
+  FULL_SIMP_TAC (std_ss++holBACore_ss++wordsLib.SIZES_ss) [reverse_endian64_ALT_DEF,
+    wordsTheory.word_shift_bv]
+));
+
+
+val _ = export_theory();
