src/tools/lifter/examples/aes-test.sml
@@ -6,15 +6,18 @@ open gcc_supportLib
 val _ = Parse.current_backend := PPBackEnd.vt100_terminal;
 val _ = set_trace "bir_inst_lifting.DEBUG_LEVEL" 2;
 
+val _ = print_with_style [Bold, Underline] "Lifting aes-aarch64.da\n";
+
 val (region_map, aes_sections) = read_disassembly_file (K true) "aes-aarch64.da"
 
 val (thm_arm8, errors) = bmil_arm8.bir_lift_prog_gen ((Arbnum.fromInt 0), (Arbnum.fromInt 0x1000000))
   aes_sections
 
-
+val _ = print "\n\n\n";
+val _ = print_with_style [Bold, Underline] "Lifting aes-m0-cortex.da\n";
 val (region_map, aes_sections) = read_disassembly_file (K true) "aes-m0-cortex.da"
 
-val (thm_m0, errors) = bmil_m0_LittleEnd_Main.bir_lift_prog_gen ((Arbnum.fromInt 0), (Arbnum.fromInt 0x10000))
+val (thm_m0, errors) = bmil_m0_LittleEnd_Process.bir_lift_prog_gen ((Arbnum.fromInt 0), (Arbnum.fromInt 0x10000))
   aes_sections
 
 val _ = print "\n\n";
